
\documentclass{article}
\usepackage{graphicx}
\usepackage{hyperref}
\usepackage{listings}
%%\usepackage{apacite}
\usepackage{helvet}
\usepackage{ragged2e}
\usepackage{titlesec}
\usepackage{courier}
%\usepackage{fontenc}
%\usepackage{fontspec}
\usepackage{amsmath}
%\usepackage{enumitem}
\usepackage[shortlabels]{enumitem}


%\lstset{basicstyle=\footnotesize\ttfamily, language=SQL}

\graphicspath{ {./images/} }

\begin{document}

    \begin{FlushLeft}
        Ian Manix

        Additional Logic Practice

        April 8, 2023
    \end{FlushLeft}

    \section*{1}

    \begin{enumerate}[a)]
      
        % 1
        \item $\exists{x}\forall{y}\; Shaves(x,y) \land Barber(x) \land Man(y)$
        \item $\exists{x}\forall{y}\; Shaves(x,y) \land Barber(x) \land Man(y) \land \neg Self\_Shave(x)$ where Self\_Shave(x) is someone who shaves themselves
        \item s $\exists{x} \forall{y}\; Shaves(x,y) \land Barber(x) \land Barber(y)$

    \end{enumerate}


    \section*{2}

    \begin{center}
    \begin{tabular} {| c | c | c | c | c | c | c |}
        \hline
        B & C & D & $B \lor C \implies D$ & $B \implies D$ & $C \implies D$ & $(B \implies D) \land (C \implies D)$ \\
        \hline
        T & T & T & T & T & T & T \\
        \hline
        T & T & F & F & F & T & F \\
        \hline
        T & F & T & T & T & F & F \\
        \hline
        T & F & F & F & F & T & F \\
        \hline
        F & T & T & T & T & T & T \\
        \hline
        F & T & F & F & T & F & F \\
        \hline
        F & F & T & T & T & T & T \\
        \hline
        F & F & F & T & T & T & T \\
        \hline
    \end{tabular}
    \end{center}
    $B \lor C \implies D$ and $(B \implies D) \land (C \implies D)$ are not logically equivalent because in the case of B=T, C=F, and D=T they do not evaluate to the same result. 


    \section*{3}
    C is true: \\
    E is true (5), this means that $D \lor B$ must be false (3) \\
    If D is false A must be true (4) \\
    Given the above two $B \implies A$ \\
    B is undefined, but:
    \begin{itemize}
        \item If B is true then C must be true as $B \implies A \implies C$ and false cannot imply true 
        \item If B in instead false then C must be true because $\neg B \implies C$ and false cannot imply true
    \end{itemize}

    

\end{document}
\endinput